proof/theories/Bytecode.v
@@ -50,6 +50,7 @@ Inductive instr : Type :=
 | IDup         (devreg addrreg : option reg)
 | IObjrefMap   (sregs : list reg) (name : string)
 | ICtSetDir    (key dir : string) (src : reg)
+| IExthdrWrite (proto : string) (htype off len : nat) (src : reg)
 | ICtDirLoad   (key dir : string) (dst : reg)
 | IXfrmLoad    (dir : string) (spnum : nat) (key : string) (dst : reg)
 | ITunnelLoad  (key : string) (dst : reg)
